Fix inferencer translation
- Noticed that check_tscheme_inst has an extra(?) first argument for
  some reason

compiler/inference/inferScript.sml
@@ -33,6 +33,40 @@ val inf_type_to_string_pmatch = Q.store_thm("inf_type_to_string_pmatch",`
   >> rpt(CONV_TAC(RAND_CONV patternMatchesLib.PMATCH_ELIM_CONV) >> every_case_tac)
   >> fs[inf_type_to_string_def]);
 
+val hex_alt_def = Define`
+  hex_alt x = (if x < 16 then HEX x else #"0")`
+
+val num_to_dec_string_alt_def = Define `num_to_dec_string_alt = n2s 10 hex_alt`;
+
+val inf_type_to_string_alt_def = tDefine"inf_type_to_string_alt"`
+(inf_type_to_string_alt (Infer_Tuvar _)=  "<unification variable>")
+/\ (inf_type_to_string_alt (Infer_Tvar_db n)=  (num_to_dec_string_alt n))
+/\ (inf_type_to_string_alt (Infer_Tapp [t1;t2] TC_fn)=
+ (STRCAT"("  (STRCAT(inf_type_to_string_alt t1)  (STRCAT"->"  (STRCAT(inf_type_to_string_alt t2) ")")))))
+/\ (inf_type_to_string_alt (Infer_Tapp ts TC_fn)=  "<bad function type>")
+/\ (inf_type_to_string_alt (Infer_Tapp ts TC_tup)=
+ (STRCAT"("  (STRCAT(inf_types_to_string_alt ts) ")")))
+/\ (inf_type_to_string_alt (Infer_Tapp [] tc1)=  (tc_to_string tc1))
+/\ (inf_type_to_string_alt (Infer_Tapp ts tc1)=
+ (STRCAT"("  (STRCAT(inf_types_to_string_alt ts)  (STRCAT") " (tc_to_string tc1)))))
+/\ (inf_types_to_string_alt []=  "")
+/\ (inf_types_to_string_alt [t]=  (inf_type_to_string_alt t))
+/\ (inf_types_to_string_alt (t::ts)=   (STRCAT(inf_type_to_string_alt t)  (STRCAT", " (inf_types_to_string_alt ts))))`
+(WF_REL_TAC `measure (\x. case x of INL x => infer_t_size x | INR x => infer_t1_size x)`>>
+rw[infer_t_size_def])
+
+val inf_type_to_string_alt_eqn = Q.store_thm("inf_type_to_string_alt_eqn",`
+  (∀t.inf_type_to_string_alt t = inf_type_to_string t) ∧
+  (∀ts.inf_types_to_string_alt ts = inf_types_to_string ts)`,
+  ho_match_mp_tac inf_type_to_string_ind>>
+  rw[inf_type_to_string_alt_def,inf_type_to_string_def,num_to_dec_string_alt_def]>>
+  fs[ASCIInumbersTheory.n2s_def,ASCIInumbersTheory.num_to_dec_string_def]>>
+  fs[MAP_EQ_f,hex_alt_def,MEM_EL]>>
+  ntac 2 strip_tac>>
+  imp_res_tac numposrepTheory.EL_n2l>>fs[]>>
+  `(n DIV 10 ** n') MOD 10 < 10` by fs[]>>
+  simp[]);
+
 val list_subset_def = Define `
 list_subset l1 l2 = EVERY (\x. MEM x l2) l1`;
 
